fi = (1 + qr5)/2
psi = (1 - qr5)/2

As the hint suggests, I will try to prove
the lemma:

(*) Fib(n) = (fi^n - psi^n)/qr5

To prove by induction, I'll first prove
the base cases:

Fib(0) = (fi^0 - psi^0)/qr5 = 0
Fib(1) = (fi^1 - psi^1)/qr5
  fi - psi = qr5 =>
  Fib(1) = qr5/qr5 = 1

Done. Now the induction step. Assuming
that the lemma (*) is true for n-1 and
n-2, I will prove that it's true for n:

Fib(n) = Fib(n-1) + Fib(n-2) =
(fi^(n-1) - psi^(n-1) + fi^(n-2) - psi^(n-2)) / qr5 =
((fi+1)*fi^(n-2) - (psi+1)*psi(n-2)) / qr5

But fi is the renown Golden Ratio, so:

fi^2 = fi+1

If you check with a calculator, you'll
see that the same can be said of psi:

(2) psi^2 = psi+1

So if we substitute fi+1 and psi+1:

(fi^2*fi^(n-2) - psi^2*psi^(n-2)) / qr5 =
(fi^n - psi^n) / qr5
Q.E.D. hint

Now, to use this hint for the final proof,
just notice that psi = -0.618, so when n
becomes large, psi becomes negligible, and
so Fib(n) can be approximated well by:

fi^n/qr5
Q.E.D.
